\documentclass{scrartcl}

% --- PREAMBLE ---
% The amsmath package is essential for professional math typesetting.
% It gives us the align* environment and the \text{} command.
\usepackage{amsmath} 
% Provides better symbols, like \coloneqq for :=
\usepackage{amssymb} 
% For better margins
\usepackage[margin=1in]{geometry}

\begin{document}
    \section*{Problems}

    % Use a standard section heading for the problems
    \section*{Problems}

    % Use the 'enumerate' environment for a numbered list of problems.
    % It handles all numbering and indentation automatically.
    \begin{enumerate}
        \item Verify the following identities by writing out (using logical symbols) what it means for an object x to be an element of each set and then using logical equivalences.
        % Use a nested enumerate for sub-problems (a), (b), etc.
        \begin{enumerate}
            \item $A \setminus (A \cap B) = A \setminus B$
            \item $A \cup (B \cap C) = (A \cup B) \cap (A \cup C)$
        \end{enumerate}

        \item Verify the following identities by writing out (using logical symbols) what it means for an object x to be an element of each set and then using logical equivalences.
        \begin{enumerate}
            \item $(A \cup B) \setminus C = (A \setminus C) \cup (B \setminus C)$
            \item $A \cup (B \setminus C) = (A \cup B) \setminus (C \setminus A)$
        \end{enumerate}
    \end{enumerate}

    \section*{Solutions}

    \subsection*{Solution to 5(a)}
    To show $A \setminus (A \cap B) = A \setminus B$, we show that for any object $x$, the statement $x \in A \setminus (A \cap B)$ is logically equivalent to $x \in A \setminus B$.

    % Use the 'align*' environment for a series of equations or equivalences. 
    % The '&' indicates where LaTeX aligns each line. 
    % The '\' starts a new line. 
    % The '*' prevents automatic line numbering numbering.
    \begin{align*}
        x \in A \setminus (A \cap B) 
        % The \Leftrightarrow symbol is often used for logical equivalence.
        &\Leftrightarrow x \in A \wedge \neg (x \in A \cap B) 
        && \text{(by definition of $\setminus$)} \\
        % The \text{} command is used for adding commentary within a math environment.
        &\Leftrightarrow x \in A \wedge \neg (x \in A \wedge x \in B)
        && \text{(by definition of $\cap$)} \\
        &\Leftrightarrow x \in A \wedge (x \notin A \vee x \notin B)
        && \text{(by De Morgan's Law)} \\
        &\Leftrightarrow (x \in A \wedge x \notin A) \vee (x \in A \wedge x \notin B)
        && \text{(by the Distributive Law)} \\
        &\Leftrightarrow \bot \vee (x \in A \wedge x \notin B)
        && \text{(by the Law of Contradiction)} \\
        &\Leftrightarrow x \in A \wedge x \notin B
        && \text{(by the Identity Law for $\vee$)} \\
        &\Leftrightarrow x \in A \setminus B
        && \text{(by definition of $\setminus$)}
    \end{align*}
    \hfill $\blacksquare$


    \subsection*{Solution to 5(b)}
    To show $A \cup (B \cap C) = (A \cup B) \cap (A \cup C)$, we show that for any object $x$, the statement $x \in A \cup (B \cap C)$ is equivalent to $x \in (A \cup B) \cap (A \cup C)$

    \subsection*{my attempt}
    \begin{align*}
        x \in A \cup (B \cap C)
        &\Leftrightarrow x \in A \vee x \in (B \cap C)
        && \text{(by definition of $\cup$)} \\
        &\Leftrightarrow x \in A \vee (x \in B \wedge x \in C)
        && \text{(by definition of $\cap$)} \\
        &\Leftrightarrow (x \in A \vee x \in B) \wedge (x \in A \vee x \in C)
        && \text{(by the Distributive Law)} \\
        &\Leftrightarrow (x \in A \vee x \in B) \cap (x \in A \vee x \in C)
        && \text{(by the Identity Law for $\wedge$) wrong!} \\
        &\Leftrightarrow x \in (A \cup B) \cap (A \cup C)
        && \text{(by the Identity Law for $\cup$) wrong!} \\
    \end{align*}
    \hfill $\blacksquare$

    \subsection*{correct}
    \begin{align*}
        x \in A \cup (B \cap C)
        &\Leftrightarrow x \in A \vee x \in (B \cap C)
        && \text{(by definition of $\cup$)} \\
        &\Leftrightarrow x \in A \vee (x \in B \wedge x \in C)
        && \text{(by definition of $\cap$)} \\
        &\Leftrightarrow (x \in A \vee x \in B) \wedge (x \in A \vee x \in C)
        && \text{(by the Distributive Law)} \\
        &\Leftrightarrow x \in (A \cup B) \wedge x \in (A \cup C)
        && \text{(by definition of $\cup$, applied twice)} \\
        &\Leftrightarrow x \in (A \cup B) \cap (A \cup C)
        && \text{(by definition of $\cap$)} \\
    \end{align*}
    \hfill $\blacksquare$

    \section*{notes for the night}
    I'm currently working discussing the problem with Gemini. I'll pick it up later. The conversation is in the openWebUI in docker.\\
    I am researching orders of operations and chewing on the mistakes of my solution.


\end{document}
